adding conversion between IEEE.float and Float.float (thanks to Fabian Hellauer); more code setup for IEEE.float

thys/IEEE_Floating_Point/Code_Float.thy
@@ -3,7 +3,8 @@
 section \<open>Code Generation Setup for Floats\<close>
 
 theory Code_Float
-imports IEEE
+  imports
+    Conversion_IEEE_Float
 begin
 
 code_printing type_constructor float \<rightharpoonup>
@@ -57,6 +58,26 @@ code_printing constant "float_sqrt :: float \<Rightarrow> float" \<rightharpoonu
   (SML) "Math.sqrt" and (OCaml) "Pervasives.sqrt"
 declare sqrt_def[code del]
 
+code_printing constant "Plus_infinity :: float" \<rightharpoonup>
+  (SML) "Real.posInf"
+declare Plus_infinity_def[code del]
+
+code_printing constant "Minus_infinity :: float" \<rightharpoonup>
+  (SML) "Real.negInf"
+declare Minus_infinity_def[code del]
+
+code_printing constant "Isnormal :: float \<Rightarrow> bool" \<rightharpoonup>
+  (SML) "Real.isNormal"
+declare [[code drop: "Isnormal"]]
+
+code_printing constant "Finite :: float \<Rightarrow> bool" \<rightharpoonup>
+  (SML) "Real.isFinite"
+declare [[code drop: "Finite"]]
+
+code_printing constant "Isnan :: float \<Rightarrow> bool" \<rightharpoonup>
+  (SML) "Real.isNan"
+declare [[code drop: "Isnan"]]
+
 text \<open>Mapping natural numbers to floats.\<close>
 fun float_of :: "nat \<Rightarrow> float"
 where
@@ -67,5 +88,57 @@ lemma "float_of 2 < float_of 3 + float_of 4"
   by eval
 
 export_code float_of in SML
+
+subsection \<open>Conversion from int\<close>
+
+definition "float_of_int i = Float (real_of_int i)"
+
+context includes integer.lifting begin
+lift_definition float_of_integer::"integer \<Rightarrow> float" is float_of_int .
+end
+
+lemma float_of_int[code]:
+  "float_of_int i = float_of_integer (integer_of_int i)"
+  by (auto simp: float_of_integer_def)
+
+code_printing
+  constant "float_of_integer :: integer \<Rightarrow> float" \<rightharpoonup> (SML) "Real.fromLargeInt"
+declare [[code drop: float_of_integer]]
+
+
+subsection \<open>Conversion to and from software floats\<close>
+
+lemma valid_man_exp_float_format:
+  "valid_man_exp float_format m e \<longleftrightarrow> \<bar>m\<bar> < 4503599627370496 \<and> - 971 < e \<and> e < 973"
+  by (simp add: valid_man_exp_def float_format_def bias_def bitlen_le_iff_power)
+
+code_printing
+  code_module "IEEE_Mantissa_Exponent" \<rightharpoonup> (SML)
+\<open>
+structure IEEE_Mantissa_Exponent =
+struct
+fun to_man_exp_float x =
+  case Real.toManExp x of {man = m, exp = e} =>
+    (Real.floor (Real.* (m, Math.pow (2.0, 53.0))), IntInf.- (e, 53))
+fun from_man_exp_float m e =
+  if IntInf.abs m < 4503599627370496 andalso ~971 < e andalso e < 973
+  then Real.fromManExp {man = Real.fromLargeInt m, exp = e}
+  else Real.posInf
+end
+\<close>
+\<comment>\<open>compare with the definitions of @{term to_man_exp_float} and @{term from_man_exp_float}
+  using @{thm valid_man_exp_float_format}\<close>
+code_printing
+  constant "to_man_exp_float :: float \<Rightarrow> integer * integer" \<rightharpoonup> (SML) "IEEE'_Mantissa'_Exponent.to'_man'_exp'_float" |
+  constant "from_man_exp_float :: integer \<Rightarrow> integer \<Rightarrow> float" \<rightharpoonup> (SML) "IEEE'_Mantissa'_Exponent.from'_man'_exp'_float"
+declare [[code drop: to_man_exp_float]]
+declare [[code drop: from_man_exp_float]]
+
+lemma
+  "\<forall>m\<in>{-10000..<10000}. \<forall>e\<in>{0..<100}. Float_of_IEEE (IEEE_of_Float (Float.Float m e)) = Float.Float m e"
+  by eval
+
+lemma "(IEEE_of_Float (Float.Float 1 1000)) \<doteq> Plus_infinity"
+  by eval
 
 end
